use only unbound variables in well-typed programs

Main.v
@@ -1,5 +1,6 @@
 From Stdlib Require Import PeanoNat.
 From Stdlib Require Import Lists.List.
+Import ListNotations.
 From Stdlib Require Export ListDef.
 
 Inductive type : Type :=
@@ -19,7 +20,6 @@ Inductive term : Type :=
 | Lam : var -> type -> term -> term
 | App : term -> term -> term
 .
-
 Notation "t '+' t'" := (Sum t t').
 Notation "'λ' x ':' tau '.' t" := (Lam x tau t) (at level 60).
 
@@ -27,8 +27,6 @@ Inductive value : term -> Prop :=
 | VNat (n : nat) : value (Nat n)
 | VLam (x : var) (tau : type) (t : term) : value (Lam x tau t)
 .
-
-Definition Gamma : Type := list (var * type).
 
 Fixpoint subst (t t' : term) (var : nat) : term :=
   match t with
@@ -39,22 +37,31 @@ Fixpoint subst (t t' : term) (var : nat) : term :=
   | App t1 t2 => App (subst t1 t' var) (subst t2 t' var)
   end
 .
+Notation "a [ b / c ]" := (subst a b c).
+
+Definition Gamma : Type := list (var * type).
+Notation "x : tau" := (x, tau) (at level 60).
+
+Definition domain (g : Gamma) : list var :=
+  map fst g.
+Notation "dom( g )" := (domain g).
 
 Inductive synty (g : Gamma) : term -> type -> Prop :=
 | TNat (n : nat) : synty g (Nat n) Natural
 | TSum (t t' : term) : synty g t Natural -> synty g t' Natural -> synty g (Sum t t') Natural
 | TVar (v : var) (tau : type) : In (v, tau) g -> synty g (Var v) tau
-| TLam (v : var) (tau tau' : type) (t : term) : synty ((v, tau) :: g) t tau' -> synty g (Lam v tau t) (Function tau tau')
+| TLam (v : var) (tau tau' : type) (t : term) : ~ In v (domain g) -> synty ((v, tau) :: g) t tau' -> synty g (Lam v tau t) (Function tau tau')
 | TApp (t t' : term) (tau tau' : type) : synty g t (Function tau tau') -> synty g t' tau -> synty g (App t t') tau'
 .
-
 Notation "g ⊢ t : tau" := (synty g t tau) (at level 60).
 
 Definition identity : term := Lam 0 Natural (Var 0).
 Example identity_typing : synty nil identity (Function Natural Natural).
 Proof.
   unfold identity.
-  apply TLam, TVar. unfold In. left. reflexivity.
+  apply TLam, TVar.
+  - auto.
+  - unfold In. left. reflexivity.
 Qed.
 
 Inductive red : term -> term -> Prop :=
@@ -65,7 +72,6 @@ Inductive red : term -> term -> Prop :=
 | RAppRight (x : var) (tau : type) (t : term) (t2 t2' : term) : red t2 t2' -> red (App (Lam x tau t) t2) (App (Lam x tau t) t2')
 | RApp (x : var) (tau : type) (t : term) (v : term) : value v -> red (App (Lam x tau t) v) (subst t v x)
 .
-
 Notation "t ↪ t'" := (red t t') (at level 60).
 
 Lemma canonicity_nat : forall t, synty nil t Natural -> value t -> exists n, t = Nat n.
@@ -91,7 +97,7 @@ Theorem progress : forall t tau, synty nil t tau -> (value t \/ exists t', red t
 Proof.
   intros t tau H.
   remember nil as g eqn:Gnil.
-  induction H as [g n|g t t' H1 IH1 H2 IH2|g v tau H|g v tau tau' t H IH|g t t' tau tau' H1 IH1 H2 IH2]; subst.
+  induction H as [g n|g t t' H1 IH1 H2 IH2|g v tau H|g v tau tau' t H1 H2 IH|g t t' tau tau' H1 IH1 H2 IH2]; subst.
   - left. apply VNat.
   - right. specialize (IH1 eq_refl). specialize (IH2 eq_refl).
     destruct IH1 as [H3|H3'], IH2 as [H4|H4'].
@@ -129,3 +135,51 @@ Proof.
       exists (App t'' t').
       now apply RAppLeft.
 Qed.
+
+Lemma preservation_subst : forall (g : Gamma) t t' x tau tau',
+  In (x, tau) g ->
+  synty g t tau' ->
+  synty nil t' tau ->
+  synty nil (subst t t' x) tau'.
+Proof.
+  intros g t t' x tau tau' H1 H2.
+  generalize dependent tau'.
+  induction t.
+  - intros tau' H2 H3. inversion H2. subst. cbn. apply TNat.
+  - intros tau' H2 H3. inversion H2. cbn.
+    specialize (IHt1 Natural H4 H3). specialize (IHt2 Natural H6 H3).
+    now apply TSum.
+  - intros tau' H2 H3. cbn. destruct (v =? x) eqn:Evx.
+    + apply Nat.eqb_eq in Evx. subst.
+      apply TVar in H1.
+      admit.
+    + admit.
+    (* + apply TVar.
+  -  *)
+  (* - intros tau' H2 H3. inversion H2. cbn.
+    specialize (IHt (Function tau0 tau')). specialize (IHt2 tau0 H5).
+    now apply TApp with (tau := tau0). *)
+Admitted.
+
+Theorem preservation : forall t tau t', synty nil t tau -> red t t' -> synty nil t' tau.
+Proof.
+  intros t tau t' H1 H2.
+  generalize dependent tau.
+  induction H2 as [
+    t1 t1' t2 H2 IH|
+    n t2 t2' H2 IH|
+    n1 n2|
+    t1 t1' t2 H2 IH|
+    x tau t t2 t2' H2 IH|
+    x tau t t2 H2].
+  - intros tau H1. specialize (IH tau).
+    inversion H1. subst. specialize (IH H3). now apply TSum.
+  - intros tau H1. specialize (IH tau).
+    inversion H1. subst. specialize (IH H5). now apply TSum.
+  - intros tau H1. inversion H1. subst. apply TNat.
+  - intros tau H1. inversion H1. subst.
+    specialize (IH (Function tau0 tau) H3).
+    now apply TApp with (tau := tau0).
+  - intros tau' H1. inversion H1. subst. specialize (IH tau0 H5).
+    now apply TApp with (tau := tau0).
+  - intros tau' H1. inversion H1. subst.
